experiment on proving a hoare rule sound

core/Hoare.v
@@ -7,6 +7,7 @@ Section Hoare.
 
 Context {tags_t: Type} {tags_t_inhabitant : Inhabitant tags_t}.
 Notation Val := (@ValueBase tags_t).
+Notation Lval := (@ValueLvalue tags_t).
 
 Notation ident := (P4String.t tags_t).
 Notation path := (list ident).
@@ -19,7 +20,25 @@ Context `{@Target tags_t (@Expression tags_t)}.
 Variable ge : (@genv tags_t).
 Variable inst_m : (@inst_mem tags_t).
 
-Definition assertion := state -> Prop.
+Definition assertion := state -> Prop. (* shallow assertion *)
+
+Definition hoare_expr (p : path) (pre : assertion) (expr : Expression) (v : Val) :=
+  forall st v',
+    pre st ->
+    exec_expr ge p st expr v' ->
+    v' = v.
+
+Definition hoare_lvalue_expr (p : path) (pre : assertion) (expr : Expression) (lv : Lval) :=
+  forall st lv' sig,
+    pre st ->
+    exec_lvalue_expr ge p st expr lv' sig ->
+    sig = SContinue /\ lv' = lv.
+
+Definition assign_lvalue (p : path) (pre : assertion) (lv : Lval) (v : Val) (post : assertion) :=
+  forall st st',
+    pre st ->
+    assign_lvalue p st lv v st' ->
+    post st'.
 
 Definition hoare_stmt (p : path) (pre : assertion) (stmt : Statement) (post : assertion) :=
   forall st st' sig,
@@ -66,12 +85,12 @@ Inductive deep_hoare_block : path -> assertion -> Block -> assertion -> Prop :=
       deep_hoare_block p mid block post ->
       deep_hoare_block p pre (BlockCons stmt block) post.
 
-Definition hoare_eval_expr (p : path) (pre : assertion) (expr : Expression) (v : Val) : Prop :=
+Definition hoare_exec_expr (p : path) (pre : assertion) (expr : Expression) (v : Val) : Prop :=
   forall st,
     pre st ->
     exec_expr ge p st expr v.
 
-Definition hoare_eval_lvalue_expr (p : path) (pre : assertion) (expr : Expression) (lv : Lval) : Prop :=
+Definition hoare_exec_lvalue_expr (p : path) (pre : assertion) (expr : Expression) (lv : Lval) : Prop :=
   forall st,
     pre st ->
     exec_lvalue_expr ge p st expr lv SContinue.
