core/ConcreteHoare.v
@@ -1,0 +1,77 @@
+Require Import Poulet4.Typed.
+Require Import Poulet4.Syntax.
+Require Import Poulet4.Semantics.
+Require Import ProD3.core.Coqlib.
+Require Import ProD3.core.Hoare.
+Require Import ProD3.core.AssertionLang.
+Require Import Hammer.Tactics.Tactics.
+
+Section ConcreteHoare.
+
+Context {tags_t: Type} {tags_t_inhabitant : Inhabitant tags_t}.
+Notation Val := (@ValueBase tags_t).
+
+Notation ident := (P4String.t tags_t).
+Notation path := (list ident).
+Notation P4Int := (P4Int.t tags_t).
+Notation P4String := (P4String.t tags_t).
+Notation signal := (@signal tags_t).
+Notation assertion := (@assertion tags_t).
+
+Context `{@Target tags_t (@Expression tags_t)}.
+
+Variable ge : (@genv tags_t).
+Variable inst_m : (@inst_mem tags_t).
+(* Variable this : path. *)
+
+Definition hoare_expr (pre : assertion) (expr : Expression) (v : Val) : Prop :=
+  eval_expr pre expr = Some v.
+
+Lemma hoare_expr_sound : forall p pre expr v,
+  hoare_expr pre expr v ->
+  Hoare.hoare_expr ge p (to_shallow_assertion p pre) expr v.
+Admitted.
+
+Definition hoare_lvalue_expr (p : path) (pre : assertion) (expr : @Expression tags_t) (lv : @Lval tags_t) : Prop :=
+  True. (* TODO *)
+
+Lemma hoare_lvalue_expr_sound : forall p pre expr lv,
+  hoare_lvalue_expr p pre expr lv ->
+  Hoare.hoare_lvalue_expr ge p (to_shallow_assertion p pre) expr lv.
+Admitted.
+
+Definition assign_lvalue (pre : assertion) (lv : @Lval tags_t) (v : Val) (post : assertion) : Prop :=
+  True. (* TODO *)
+
+Lemma assign_lvalue_sound : forall p pre lv v post,
+  assign_lvalue pre lv v post ->
+  Hoare.assign_lvalue p (to_shallow_assertion p pre) lv v (to_shallow_assertion p post).
+Admitted.
+
+Inductive hoare_stmt : path -> assertion -> (@Statement tags_t) -> assertion -> Prop :=
+  | hoare_stmt_assignment : forall p pre tags lhs rhs typ post lv v,
+      hoare_lvalue_expr p pre lhs lv ->
+      hoare_expr pre rhs v ->
+      assign_lvalue pre lv v post ->
+      hoare_stmt p pre (MkStatement tags (StatAssignment lhs rhs) typ) post.
+
+Lemma hoare_stmt_sound : forall p pre stmt post,
+  hoare_stmt p pre stmt post ->
+  Hoare.hoare_stmt ge inst_m p (to_shallow_assertion p pre) stmt (to_shallow_assertion p post).
+Proof.
+  intros * H_hoare_stmt.
+  induction H_hoare_stmt.
+  - repeat lazymatch goal with
+    | H : hoare_lvalue_expr _ _ _ _ |- _ => apply hoare_lvalue_expr_sound in H
+    | H : hoare_expr _ _ _ |- _ => apply hoare_expr_sound with (p := p) in H
+    | H : assign_lvalue _ _ _ _ |- _ => eapply assign_lvalue_sound with (p := p) in H
+    end.
+    hnf. intros. inversion H4.
+    + hauto unfold: Hoare.assign_lvalue, Hoare.hoare_expr, Hoare.hoare_lvalue_expr.
+    + admit. (* assign call rule should be ruled out, but we cnanot prove it now. *)
+    + admit. (* assign call rule should be ruled out, but we cnanot prove it now. *)
+    + unfold Hoare.hoare_lvalue_expr in H0. hauto lq: on.
+(* Qed. *)
+Admitted.
+
+End ConcreteHoare.
